lib/Lib.Exponentiation.Definition.fst
@@ -18,13 +18,13 @@ val lemma_mul_cancel_inverse: #t:Type -> k:abelian_group t -> a:t -> b:t ->
 let lemma_mul_cancel_inverse #t k a b =
   calc (==) {
     cm.mul (inverse a) (cm.mul a b);
-    (==) { cm.lemma_mul_assoc (inverse a) a b }
+    == { cm.lemma_mul_assoc (inverse a) a b }
     cm.mul (cm.mul (inverse a) a) b;
-    (==) { lemma_inverse a }
+    == { lemma_inverse a }
     cm.mul cm.one b;
-    (==) { cm.lemma_mul_comm cm.one b }
+    == { cm.lemma_mul_comm cm.one b }
     cm.mul b cm.one;
-    (==) { cm.lemma_one b }
+    == { cm.lemma_one b }
     b;
   }
 
@@ -54,15 +54,15 @@ let lemma_inverse_mul #t k a b =
   assert (cm.mul (cm.mul a b) (inverse (cm.mul a b)) == cm.one);
   calc (==) {
     cm.mul (cm.mul a b) (cm.mul (inverse a) (inverse b));
-    (==) { cm.lemma_mul_assoc (cm.mul a b) (inverse a) (inverse b) }
+    == { cm.lemma_mul_assoc (cm.mul a b) (inverse a) (inverse b) }
     cm.mul (cm.mul (cm.mul a b) (inverse a)) (inverse b);
-    (==) { cm.lemma_mul_comm (cm.mul a b) (inverse a) }
+    == { cm.lemma_mul_comm (cm.mul a b) (inverse a) }
     cm.mul (cm.mul (inverse a) (cm.mul a b)) (inverse b);
-    (==) { lemma_mul_cancel_inverse k a b }
+    == { lemma_mul_cancel_inverse k a b }
     cm.mul b (inverse b);
-    (==) { cm.lemma_mul_comm b (inverse b) }
+    == { cm.lemma_mul_comm b (inverse b) }
     cm.mul (inverse b) b;
-    (==) { lemma_inverse b }
+    == { lemma_inverse b }
     cm.one;
   };
 
@@ -97,23 +97,23 @@ let rec lemma_pow_add #t k x n m =
   if n = 0 then begin
     calc (==) {
       mul (pow k x n) (pow k x m);
-      (==) { lemma_pow0 k x }
+      == { lemma_pow0 k x }
       mul one (pow k x m);
-      (==) { lemma_mul_comm one (pow k x m) }
+      == { lemma_mul_comm one (pow k x m) }
       mul (pow k x m) one;
-      (==) { lemma_one (pow k x m) }
+      == { lemma_one (pow k x m) }
       pow k x m;
       }; () end
   else begin
     calc (==) {
       mul (pow k x n) (pow k x m);
-      (==) { lemma_pow_unfold k x n }
+      == { lemma_pow_unfold k x n }
       mul (mul x (pow k x (n - 1))) (pow k x m);
-      (==) { lemma_mul_assoc x (pow k x (n - 1)) (pow k x m) }
+      == { lemma_mul_assoc x (pow k x (n - 1)) (pow k x m) }
       mul x (mul (pow k x (n - 1)) (pow k x m));
-      (==) { lemma_pow_add #t k x (n - 1) m }
+      == { lemma_pow_add #t k x (n - 1) m }
       mul x (pow k x (n - 1 + m));
-      (==) { lemma_pow_unfold k x (n + m) }
+      == { lemma_pow_unfold k x (n + m) }
       pow k x (n + m);
       }; () end
 
@@ -126,11 +126,11 @@ let rec lemma_pow_mul #t k x n m =
   else begin
     calc (==) {
       pow k (pow k x n) m;
-      (==) { lemma_pow_unfold k (pow k x n) m }
+      == { lemma_pow_unfold k (pow k x n) m }
       mul (pow k x n) (pow k (pow k x n) (m - 1));
-      (==) { lemma_pow_mul k x n (m - 1) }
+      == { lemma_pow_mul k x n (m - 1) }
       mul (pow k x n) (pow k x (n * (m - 1)));
-      (==) { lemma_pow_add k x n (n * (m - 1)) }
+      == { lemma_pow_add k x n (n * (m - 1)) }
       pow k x (n * m);
     }; () end
 
@@ -144,19 +144,19 @@ let rec lemma_pow_mul_base #t k a b n =
   else begin
     calc (==) {
       mul (pow k a n) (pow k b n);
-      (==) { lemma_pow_unfold k a n; lemma_pow_unfold k b n }
+      == { lemma_pow_unfold k a n; lemma_pow_unfold k b n }
       mul (mul a (pow k a (n - 1))) (mul b (pow k b (n - 1)));
-      (==) { lemma_mul_comm b (pow k b (n - 1));
+      == { lemma_mul_comm b (pow k b (n - 1));
        lemma_mul_assoc a (pow k a (n - 1)) (mul (pow k b (n - 1)) b) }
       mul a (mul (pow k a (n - 1)) (mul (pow k b (n - 1)) b));
-      (==) { lemma_mul_assoc (pow k a (n - 1)) (pow k b (n - 1)) b }
+      == { lemma_mul_assoc (pow k a (n - 1)) (pow k b (n - 1)) b }
       mul a (mul (mul (pow k a (n - 1)) (pow k b (n - 1))) b);
-      (==) { lemma_pow_mul_base #t k a b (n - 1) }
+      == { lemma_pow_mul_base #t k a b (n - 1) }
       mul a (mul (pow k (mul a b) (n - 1)) b);
-      (==) { lemma_mul_comm (pow k (mul a b) (n - 1)) b;
+      == { lemma_mul_comm (pow k (mul a b) (n - 1)) b;
 	lemma_mul_assoc a b (pow k (mul a b) (n - 1)) }
       mul (mul a b) (pow k (mul a b) (n - 1));
-      (==) { lemma_pow_unfold k (mul a b) n }
+      == { lemma_pow_unfold k (mul a b) n }
       pow k (mul a b) n;
     }; () end
 
@@ -164,9 +164,9 @@ let rec lemma_pow_mul_base #t k a b n =
 let lemma_pow_double #t k x b =
   calc (==) {
     pow k (mul x x) b;
-    (==) { lemma_pow_mul_base k x x b}
+    == { lemma_pow_mul_base k x x b}
     mul (pow k x b) (pow k x b);
-    (==) { lemma_pow_add k x b b }
+    == { lemma_pow_add k x b b }
     pow k x (b + b);
     }
 
@@ -181,13 +181,13 @@ let rec lemma_inverse_pow #t k x n =
   else begin
     calc (==) {
       k.inverse (pow k.cm x n);
-      (==) { lemma_pow_unfold k.cm x n }
+      == { lemma_pow_unfold k.cm x n }
       k.inverse (k.cm.mul x (pow k.cm x (n - 1)));
-      (==) { lemma_inverse_mul k x (pow k.cm x (n - 1)) }
+      == { lemma_inverse_mul k x (pow k.cm x (n - 1)) }
       k.cm.mul (k.inverse x) (k.inverse (pow k.cm x (n - 1)));
-      (==) { lemma_inverse_pow k x (n - 1) }
+      == { lemma_inverse_pow k x (n - 1) }
       k.cm.mul (k.inverse x) (pow k.cm (k.inverse x) (n - 1));
-      (==) { lemma_pow_unfold k.cm (inverse x) n }
+      == { lemma_pow_unfold k.cm (inverse x) n }
       pow k.cm (k.inverse x) n;
     } end
 
@@ -210,31 +210,31 @@ let lemma_pow_neg_add_aux #t k x n m =
   if -n <= m then begin
   calc (==) {
     k.cm.mul (k.inverse (pow k.cm x (-n))) (pow k.cm x m);
-    (==) { lemma_pow_add k.cm x (-n) (m + n) }
+    == { lemma_pow_add k.cm x (-n) (m + n) }
     k.cm.mul (k.inverse (pow k.cm x (-n))) (k.cm.mul (pow k.cm x (-n)) (pow k.cm x (m + n)));
-    (==) { k.cm.lemma_mul_assoc
+    == { k.cm.lemma_mul_assoc
       (k.inverse (pow k.cm x (-n))) (pow k.cm x (-n)) (pow k.cm x (m + n)) }
     k.cm.mul (k.cm.mul (k.inverse (pow k.cm x (- n))) (pow k.cm x (-n))) (pow k.cm x (m + n));
-    (==) { k.lemma_inverse (pow k.cm x (- n)) }
+    == { k.lemma_inverse (pow k.cm x (- n)) }
     k.cm.mul k.cm.one (pow k.cm x (m + n));
-    (==) { k.cm.lemma_mul_comm k.cm.one (pow k.cm x (m + n)) }
+    == { k.cm.lemma_mul_comm k.cm.one (pow k.cm x (m + n)) }
     k.cm.mul (pow k.cm x (m + n)) k.cm.one;
-    (==) { k.cm.lemma_one (pow k.cm x (m + n)) }
+    == { k.cm.lemma_one (pow k.cm x (m + n)) }
     pow k.cm x (m + n);
   } end
   else begin
   calc (==) {
     k.cm.mul (k.inverse (pow k.cm x (-n))) (pow k.cm x m);
-    (==) { lemma_pow_add k.cm x (-n-m) m }
+    == { lemma_pow_add k.cm x (-n-m) m }
     k.cm.mul (k.inverse (k.cm.mul (pow k.cm x (-n-m)) (pow k.cm x m))) (pow k.cm x m);
-    (==) { lemma_inverse_mul k (pow k.cm x (-n-m)) (pow k.cm x m) }
+    == { lemma_inverse_mul k (pow k.cm x (-n-m)) (pow k.cm x m) }
     k.cm.mul (k.cm.mul (k.inverse (pow k.cm x (-n-m))) (k.inverse (pow k.cm x m))) (pow k.cm x m);
-    (==) { k.cm.lemma_mul_assoc
+    == { k.cm.lemma_mul_assoc
       (k.inverse (pow k.cm x (-n-m))) (k.inverse (pow k.cm x m)) (pow k.cm x m) }
     k.cm.mul (k.inverse (pow k.cm x (-n-m))) (k.cm.mul (k.inverse (pow k.cm x m)) (pow k.cm x m));
-    (==) { k.lemma_inverse (pow k.cm x m) }
+    == { k.lemma_inverse (pow k.cm x m) }
     k.cm.mul (k.inverse (pow k.cm x (-n-m))) k.cm.one;
-    (==) { k.cm.lemma_one (k.inverse (pow k.cm x (-n-m))) }
+    == { k.cm.lemma_one (k.inverse (pow k.cm x (-n-m))) }
     k.inverse (pow k.cm x (-n-m));
   } end
 
@@ -246,11 +246,11 @@ let lemma_pow_neg_add #t k x n m =
     if n < 0 && m < 0 then begin
       calc (==) {
         k.cm.mul (pow_neg k x n) (pow_neg k x m);
-        (==) { }
+        == { }
         k.cm.mul (k.inverse (pow k.cm x (- n))) (k.inverse (pow k.cm x (- m)));
-        (==) { lemma_inverse_mul k (pow k.cm x (- n)) (pow k.cm x (- m)) }
+        == { lemma_inverse_mul k (pow k.cm x (- n)) (pow k.cm x (- m)) }
         k.inverse (k.cm.mul (pow k.cm x (- n)) (pow k.cm x (- m)));
-        (==) { lemma_pow_add k.cm x (- n) (- m) }
+        == { lemma_pow_add k.cm x (- n) (- m) }
         k.inverse (pow k.cm x (- n - m));
       } end
     else begin
@@ -294,11 +294,11 @@ val lemma_pow_neg_mul_nneg: #t:Type -> k:abelian_group t -> x:t -> n:int -> m:in
 let lemma_pow_neg_mul_nneg #t k x n m =
   calc (==) {
     pow_neg k (pow_neg k x n) m;
-    (==) { }
+    == { }
     pow k.cm (k.inverse (pow k.cm x (-n))) m;
-    (==) { lemma_inverse_pow k (pow k.cm x (-n)) m }
+    == { lemma_inverse_pow k (pow k.cm x (-n)) m }
     k.inverse (pow k.cm (pow k.cm x (-n)) m);
-    (==) { lemma_pow_mul k.cm x (-n) m }
+    == { lemma_pow_mul k.cm x (-n) m }
     k.inverse (pow k.cm x (-n * m));
   }
 
@@ -310,9 +310,9 @@ val lemma_pow_neg_mul_mneg: #t:Type -> k:abelian_group t -> x:t -> n:int -> m:in
 let lemma_pow_neg_mul_mneg #t k x n m =
   calc (==) {
     pow_neg k (pow_neg k x n) m;
-    (==) { }
+    == { }
     k.inverse (pow k.cm (pow k.cm x n) (-m));
-    (==) { lemma_pow_mul k.cm x n (-m) }
+    == { lemma_pow_mul k.cm x n (-m) }
     k.inverse (pow k.cm x (-n * m));
   }
 
@@ -324,13 +324,13 @@ let lemma_pow_neg_mul #t k x n m =
     if n < 0 && m < 0 then
     calc (==) {
       pow_neg k (pow_neg k x n) m;
-      (==) { }
+      == { }
       k.inverse (pow k.cm (k.inverse (pow k.cm x (-n))) (-m));
-      (==) { lemma_inverse_pow k (pow k.cm x (-n)) (-m) }
+      == { lemma_inverse_pow k (pow k.cm x (-n)) (-m) }
       k.inverse (k.inverse (pow k.cm (pow k.cm x (-n)) (-m)));
-      (==) { lemma_inverse_id k (pow k.cm (pow k.cm x (-n)) (-m)) }
+      == { lemma_inverse_id k (pow k.cm (pow k.cm x (-n)) (-m)) }
       pow k.cm (pow k.cm x (-n)) (-m);
-      (==) { lemma_pow_mul k.cm x (-n) (-m) }
+      == { lemma_pow_mul k.cm x (-n) (-m) }
       pow k.cm x (n * m);
     }
     else begin
@@ -349,11 +349,11 @@ let lemma_pow_neg_mul_base #t k a b n =
   else begin
     calc (==) {
       k.cm.mul (pow_neg k a n) (pow_neg k b n);
-      (==) { }
+      == { }
       k.cm.mul (k.inverse (pow k.cm a (-n))) (k.inverse (pow k.cm b (-n)));
-      (==) { lemma_inverse_mul k (pow k.cm a (-n)) (pow k.cm b (-n)) }
+      == { lemma_inverse_mul k (pow k.cm a (-n)) (pow k.cm b (-n)) }
       k.inverse (k.cm.mul (pow k.cm a (-n)) (pow k.cm b (-n)));
-      (==) { lemma_pow_mul_base k.cm a b (- n) }
+      == { lemma_pow_mul_base k.cm a b (- n) }
       k.inverse (pow k.cm (k.cm.mul a b) (-n));
      } end
 
@@ -361,8 +361,8 @@ let lemma_pow_neg_mul_base #t k a b n =
 let lemma_pow_neg_double #t k x b =
   calc (==) {
     pow_neg k (k.cm.mul x x) b;
-    (==) { lemma_pow_neg_mul_base k x x b}
+    == { lemma_pow_neg_mul_base k x x b}
     k.cm.mul (pow_neg k x b) (pow_neg k x b);
-    (==) { lemma_pow_neg_add k x b b }
+    == { lemma_pow_neg_add k x b b }
     pow_neg k x (b + b);
   }
